theories/typing/function.v
@@ -210,7 +210,7 @@ Section typing.
     rewrite -typed_body_mono /flip; last done; first by eapply type_call.
     - etrans. eapply (incl_cctx_incl _ [_]); first by intros ? ->%elem_of_list_singleton.
       apply cctx_incl_cons_match; first done. intros args. inv_vec args=>ret q. inv_vec q. done.
-    - etrans; last by apply (tctx_incl_frame_l _ _ [_]).
+    - etrans; last by apply (tctx_incl_frame_l [_]).
       apply copy_elem_of_tctx_incl; last done. apply _.
   Qed.
 
